examples/n_german/nGerman.thy
@@ -23,11 +23,11 @@ definition false :: scalrValueType where [simp]: "false \<equiv> boolV False"
 
 definition n_RecvGntE :: "nat \<Rightarrow> rule" where
   "n_RecvGntE i \<equiv>
-    let g = IVar (Para ''Chan2.Cmd'' i) =\<^sub>f Const GntE in
-    let a = assign (Para ''Cache.State'' i, Const E) ||
-            assign (Para ''Cache.Data'' i, IVar (Para ''Chan2.Data'' i)) ||
-            assign (Para ''Chan2.Cmd'' i, Const Empty) in
-      (guard g a)"
+    IVar (Para ''Chan2.Cmd'' i) =\<^sub>f Const GntE
+   \<triangleright>
+    assign (Para ''Cache.State'' i, Const E) ||
+    assign (Para ''Cache.Data'' i, IVar (Para ''Chan2.Data'' i)) ||
+    assign (Para ''Chan2.Cmd'' i, Const Empty)"
 
 lemma symRecvGntE:
   "symParamRule N n_RecvGntE"
@@ -49,11 +49,11 @@ lemma absRecvGntEAct:
 
 definition n_RecvGntS :: "nat \<Rightarrow> rule" where
   "n_RecvGntS i \<equiv>
-    let g = IVar (Para ''Chan2.Cmd'' i) =\<^sub>f Const GntS in
-    let a = assign (Para ''Cache.State'' i, Const S) ||
-            assign (Para ''Cache.Data'' i, IVar (Para ''Chan2.Data'' i)) ||
-            assign (Para ''Chan2.Cmd'' i, Const Empty) in
-      (guard g a)"
+    IVar (Para ''Chan2.Cmd'' i) =\<^sub>f Const GntS
+   \<triangleright>
+    assign (Para ''Cache.State'' i, Const S) ||
+    assign (Para ''Cache.Data'' i, IVar (Para ''Chan2.Data'' i)) ||
+    assign (Para ''Chan2.Cmd'' i, Const Empty)"
 
 lemma symRecvGntS:
   "symParamRule N n_RecvGntS"
@@ -75,23 +75,24 @@ lemma absRecvGntSAct:
 
 definition n_SendGntE :: "nat \<Rightarrow> nat \<Rightarrow> rule" where
   "n_SendGntE N i \<equiv>
-    let g = IVar (Ident ''CurCmd'') =\<^sub>f Const ReqE \<and>\<^sub>f
-            IVar (Ident ''CurPtr'') =\<^sub>f Const (index i) \<and>\<^sub>f
-            IVar (Para ''Chan2.Cmd'' i) =\<^sub>f Const Empty \<and>\<^sub>f
-            IVar (Ident ''ExGntd'') =\<^sub>f Const false \<and>\<^sub>f
-            (\<forall>\<^sub>fj. IVar (Para ''ShrSet'' j) =\<^sub>f Const false) N in
-    let a = assign (Para ''Chan2.Cmd'' i, Const GntE) ||
-            assign (Para ''Chan2.Data'' i, IVar (Ident ''MemData'')) ||
-            assign (Para ''ShrSet'' i, Const true) ||
-            assign (Ident ''ExGntd'', Const true) ||
-            assign (Ident ''CurCmd'', Const Empty) in
-      (guard g a)"
+    IVar (Ident ''CurCmd'') =\<^sub>f Const ReqE \<and>\<^sub>f
+    IVar (Ident ''CurPtr'') =\<^sub>f Const (index i) \<and>\<^sub>f
+    IVar (Para ''Chan2.Cmd'' i) =\<^sub>f Const Empty \<and>\<^sub>f
+    IVar (Ident ''ExGntd'') =\<^sub>f Const false \<and>\<^sub>f
+    (\<forall>\<^sub>fj. IVar (Para ''ShrSet'' j) =\<^sub>f Const false) N
+   \<triangleright>
+    assign (Para ''Chan2.Cmd'' i, Const GntE) ||
+    assign (Para ''Chan2.Data'' i, IVar (Ident ''MemData'')) ||
+    assign (Para ''ShrSet'' i, Const true) ||
+    assign (Ident ''ExGntd'', Const true) ||
+    assign (Ident ''CurCmd'', Const Empty)"
 
 lemma symSendGntE:
-  "symParamForm N (\<lambda>i. pre (n_SendGntE N i))"
+  "symParamRule N (n_SendGntE N)"
   unfolding n_SendGntE_def
+  apply (rule symParamRuleI)
   apply (auto intro!: symParamFormAnd symParamFormForall)
-  unfolding symParamForm_def symParamForm2_def by auto
+  unfolding symParamForm_def symParamForm2_def symParamStatement_def by auto
 
 lemma absSendGntE:
   assumes "M \<le> N"
@@ -129,15 +130,21 @@ lemma SendGntEWellForm:
 
 definition n_SendGntS :: "nat \<Rightarrow> rule" where
   "n_SendGntS i \<equiv>
-    let g = IVar (Ident ''CurCmd'') =\<^sub>f Const ReqS \<and>\<^sub>f
-            IVar (Ident ''CurPtr'') =\<^sub>f Const (index i) \<and>\<^sub>f
-            IVar (Para ''Chan2.Cmd'' i) =\<^sub>f Const Empty \<and>\<^sub>f
-            IVar (Ident ''ExGntd'') =\<^sub>f Const false in
-    let a = assign (Para ''Chan2.Cmd'' i, Const GntS) ||
-            assign (Para ''Chan2.Data'' i, IVar (Ident ''MemData'')) ||
-            assign (Para ''ShrSet'' i, Const true) ||
-            assign (Ident ''CurCmd'', Const Empty) in
-      (guard g a)"
+    IVar (Ident ''CurCmd'') =\<^sub>f Const ReqS \<and>\<^sub>f
+    IVar (Ident ''CurPtr'') =\<^sub>f Const (index i) \<and>\<^sub>f
+    IVar (Para ''Chan2.Cmd'' i) =\<^sub>f Const Empty \<and>\<^sub>f
+    IVar (Ident ''ExGntd'') =\<^sub>f Const false
+   \<triangleright>
+    assign (Para ''Chan2.Cmd'' i, Const GntS) ||
+    assign (Para ''Chan2.Data'' i, IVar (Ident ''MemData'')) ||
+    assign (Para ''ShrSet'' i, Const true) ||
+    assign (Ident ''CurCmd'', Const Empty)"
+
+lemma symSendGntS:
+  "symParamRule N n_SendGntS"
+  unfolding n_SendGntS_def
+  apply (rule symParamRuleI)
+  by (auto simp add: symParamForm_def symParamStatement_def)
 
 lemma absSendGntS:
   "absTransfForm M (pre (n_SendGntS i)) =
@@ -169,13 +176,17 @@ lemma SendGntSWellForm:
 
 definition n_RecvInvAck1 :: "nat \<Rightarrow> rule" where
   "n_RecvInvAck1 i \<equiv>
-    let g = IVar (Para ''Chan3.Cmd'' i) =\<^sub>f Const InvAck \<and>\<^sub>f
-            \<not>\<^sub>f IVar (Ident ''CurCmd'') =\<^sub>f Const Empty \<and>\<^sub>f
-            IVar (Ident ''ExGntd'') =\<^sub>f Const true in
-    let a = assign (Para ''Chan3.Cmd'' i, Const Empty) ||
-            assign (Para ''ShrSet'' i, Const false) ||
-            assign (Ident ''ExGntd'', Const false) in
-      (guard g a)"
+    IVar (Para ''Chan3.Cmd'' i) =\<^sub>f Const InvAck \<and>\<^sub>f
+    \<not>\<^sub>f IVar (Ident ''CurCmd'') =\<^sub>f Const Empty \<and>\<^sub>f
+    IVar (Ident ''ExGntd'') =\<^sub>f Const true
+   \<triangleright>
+    assign (Para ''Chan3.Cmd'' i, Const Empty) ||
+    assign (Para ''ShrSet'' i, Const false) ||
+    assign (Ident ''ExGntd'', Const false)"
+
+lemma symRecvInvAck1:
+  "symParamRule N (n_RecvInvAck1)"
+  unfolding n_RecvInvAck1_def unfolding symParamRule_def by auto
 
 lemma absRecvInvAck1:
   "absTransfForm M (pre (n_RecvInvAck1 i)) =
@@ -204,12 +215,16 @@ lemma RecvInvAck1WellForm:
 
 definition n_RecvInvAck2 :: "nat \<Rightarrow> rule" where
   "n_RecvInvAck2 i \<equiv>
-    let g = IVar (Para ''Chan3.Cmd'' i) =\<^sub>f Const InvAck \<and>\<^sub>f
-            \<not>\<^sub>f IVar (Ident ''CurCmd'') =\<^sub>f Const Empty \<and>\<^sub>f
-            \<not>\<^sub>f IVar (Ident ''ExGntd'') =\<^sub>f Const true in
-    let a = assign (Para ''Chan3.Cmd'' i, Const Empty) ||
-            assign (Para ''ShrSet'' i, Const false) in
-      (guard g a)"
+    IVar (Para ''Chan3.Cmd'' i) =\<^sub>f Const InvAck \<and>\<^sub>f
+    \<not>\<^sub>f IVar (Ident ''CurCmd'') =\<^sub>f Const Empty \<and>\<^sub>f
+    \<not>\<^sub>f IVar (Ident ''ExGntd'') =\<^sub>f Const true
+   \<triangleright>
+    assign (Para ''Chan3.Cmd'' i, Const Empty) ||
+    assign (Para ''ShrSet'' i, Const false)"
+
+lemma symRecvInvAck2:
+  "symParamRule N n_RecvInvAck2"
+  unfolding n_RecvInvAck2_def symParamRule_def by auto
 
 lemma absRecvInvAck2:
   "absTransfForm M (pre (n_RecvInvAck2 i)) =
@@ -237,14 +252,18 @@ lemma RecvInvAck2WellForm:
 
 definition n_SendInvAck1 :: "nat \<Rightarrow> rule" where
   "n_SendInvAck1 i \<equiv>
-    let g = IVar (Para ''Chan2.Cmd'' i) =\<^sub>f Const Inv \<and>\<^sub>f
-            IVar (Para ''Chan3.Cmd'' i) =\<^sub>f Const Empty \<and>\<^sub>f
-            IVar (Para ''Cache.State'' i) =\<^sub>f Const E in
-    let a = assign (Para ''Chan2.Cmd'' i, Const Empty) ||
-            assign (Para ''Chan3.Cmd'' i, Const InvAck) ||
-            assign (Para ''Chan3.Data'' i, IVar (Para ''Cache.Data'' i)) ||
-            assign (Para ''Cache.State'' i, Const I) in
-      (guard g a)"
+    IVar (Para ''Chan2.Cmd'' i) =\<^sub>f Const Inv \<and>\<^sub>f
+    IVar (Para ''Chan3.Cmd'' i) =\<^sub>f Const Empty \<and>\<^sub>f
+    IVar (Para ''Cache.State'' i) =\<^sub>f Const E
+   \<triangleright>
+    assign (Para ''Chan2.Cmd'' i, Const Empty) ||
+    assign (Para ''Chan3.Cmd'' i, Const InvAck) ||
+    assign (Para ''Chan3.Data'' i, IVar (Para ''Cache.Data'' i)) ||
+    assign (Para ''Cache.State'' i, Const I)"
+
+lemma symSendInvAck1:
+  "symParamRule N n_SendInvAck1"
+  unfolding n_SendInvAck1_def symParamRule_def by auto
 
 lemma absSendInvAck1:
   "absTransfForm M (pre (n_SendInvAck1 i)) =
@@ -273,13 +292,17 @@ lemma SendInvAck1WellForm:
 
 definition n_SendInvAck2 :: "nat \<Rightarrow> rule" where
   "n_SendInvAck2 i \<equiv>
-    let g = IVar (Para ''Chan2.Cmd'' i) =\<^sub>f Const Inv \<and>\<^sub>f
-            IVar (Para ''Chan3.Cmd'' i) =\<^sub>f Const Empty \<and>\<^sub>f
-            \<not>\<^sub>f IVar (Para ''Cache.State'' i) =\<^sub>f Const E in
-    let a = assign (Para ''Chan2.Cmd'' i, Const Empty) ||
-            assign (Para ''Chan3.Cmd'' i, Const InvAck) ||
-            assign (Para ''Cache.State'' i, Const I) in
-      (guard g a)"
+    IVar (Para ''Chan2.Cmd'' i) =\<^sub>f Const Inv \<and>\<^sub>f
+    IVar (Para ''Chan3.Cmd'' i) =\<^sub>f Const Empty \<and>\<^sub>f
+    \<not>\<^sub>f IVar (Para ''Cache.State'' i) =\<^sub>f Const E
+   \<triangleright>
+    assign (Para ''Chan2.Cmd'' i, Const Empty) ||
+    assign (Para ''Chan3.Cmd'' i, Const InvAck) ||
+    assign (Para ''Cache.State'' i, Const I)"
+
+lemma symSendInvAck2:
+  "symParamRule N n_SendInvAck2"
+  unfolding n_SendInvAck2_def symParamRule_def by auto
 
 lemma absSendInvAck2:
   "absTransfForm M (pre (n_SendInvAck2 i)) =
@@ -307,12 +330,16 @@ lemma SendInvAck2WellForm:
 
 definition n_SendInv1 :: "nat \<Rightarrow> rule" where
   "n_SendInv1 i \<equiv>
-    let g = IVar (Para ''Chan2.Cmd'' i) =\<^sub>f Const Empty \<and>\<^sub>f
-            IVar (Para ''InvSet'' i) =\<^sub>f Const true \<and>\<^sub>f
-            IVar (Ident ''CurCmd'') =\<^sub>f Const ReqE in
-    let a = assign (Para ''Chan2.Cmd'' i, Const Inv) ||
-            assign (Para ''InvSet'' i, Const false) in
-      (guard g a)"
+    IVar (Para ''Chan2.Cmd'' i) =\<^sub>f Const Empty \<and>\<^sub>f
+    IVar (Para ''InvSet'' i) =\<^sub>f Const true \<and>\<^sub>f
+    IVar (Ident ''CurCmd'') =\<^sub>f Const ReqE
+   \<triangleright>
+    assign (Para ''Chan2.Cmd'' i, Const Inv) ||
+    assign (Para ''InvSet'' i, Const false)"
+
+lemma symSendInv1:
+  "symParamRule N n_SendInv1"
+  unfolding n_SendInv1_def symParamRule_def by auto
 
 lemma absSendInv1:
   "absTransfForm M (pre (n_SendInv1 i)) =
@@ -339,13 +366,17 @@ lemma SendInv1WellForm:
 
 definition n_SendInv2 :: "nat \<Rightarrow> rule" where
   "n_SendInv2 i \<equiv>
-    let g = IVar (Para ''Chan2.Cmd'' i) =\<^sub>f Const Empty \<and>\<^sub>f
-            IVar (Para ''InvSet'' i) =\<^sub>f Const true \<and>\<^sub>f
-            IVar (Ident ''CurCmd'') =\<^sub>f Const ReqS \<and>\<^sub>f
-            IVar (Ident ''ExGntd'') =\<^sub>f Const true in
-    let a = assign (Para ''Chan2.Cmd'' i, Const Inv) ||
-            assign (Para ''InvSet'' i, Const false) in
-      (guard g a)"
+    IVar (Para ''Chan2.Cmd'' i) =\<^sub>f Const Empty \<and>\<^sub>f
+    IVar (Para ''InvSet'' i) =\<^sub>f Const true \<and>\<^sub>f
+    IVar (Ident ''CurCmd'') =\<^sub>f Const ReqS \<and>\<^sub>f
+    IVar (Ident ''ExGntd'') =\<^sub>f Const true
+   \<triangleright>
+    assign (Para ''Chan2.Cmd'' i, Const Inv) ||
+    assign (Para ''InvSet'' i, Const false)"
+
+lemma symSendInv2:
+  "symParamRule N n_SendInv2"
+  unfolding n_SendInv2_def symParamRule_def by auto
 
 lemma absSendInv2:
   "absTransfForm M (pre (n_SendInv2 i)) =
@@ -374,13 +405,22 @@ lemma SendInv2WellForm:
 
 definition n_RecvReqE :: "nat \<Rightarrow> nat \<Rightarrow> rule" where
   "n_RecvReqE N i \<equiv>
-    let g = IVar (Ident ''CurCmd'') =\<^sub>f Const Empty \<and>\<^sub>f
-            IVar (Para ''Chan1.Cmd'' i) =\<^sub>f Const ReqE in
-    let a = assign (Ident ''CurCmd'', Const ReqE) ||
-            assign (Ident ''CurPtr'', Const (index i)) ||
-            assign (Para ''Chan1.Cmd'' i, Const Empty) ||
-            forallStm (\<lambda>j. assign (Para ''InvSet'' j, IVar (Para ''ShrSet'' j))) N in
-      (guard g a)"
+    IVar (Ident ''CurCmd'') =\<^sub>f Const Empty \<and>\<^sub>f
+    IVar (Para ''Chan1.Cmd'' i) =\<^sub>f Const ReqE
+   \<triangleright>
+    assign (Ident ''CurCmd'', Const ReqE) ||
+    assign (Ident ''CurPtr'', Const (index i)) ||
+    assign (Para ''Chan1.Cmd'' i, Const Empty) ||
+    forallStm (\<lambda>j. assign (Para ''InvSet'' j, IVar (Para ''ShrSet'' j))) N"
+
+lemma symRecvReqE:
+  "symParamRule N (n_RecvReqE N)"
+  unfolding n_RecvReqE_def
+  apply (rule symParamRuleI)
+  subgoal unfolding symParamForm_def by auto
+  subgoal apply (auto intro!: symParamStatementParallel symParamStatementForall)
+    unfolding symParamStatement_def symParamStatement2_def by auto
+  done
 
 lemma absRecvReqE:
   "absTransfForm M (pre (n_RecvReqE N i)) =
@@ -410,13 +450,22 @@ lemma RecvReqEWellForm:
 
 definition n_RecvReqS :: "nat \<Rightarrow> nat \<Rightarrow> rule" where
   "n_RecvReqS N i \<equiv>
-    let g = IVar (Ident ''CurCmd'') =\<^sub>f Const Empty \<and>\<^sub>f
-            IVar (Para ''Chan1.Cmd'' i) =\<^sub>f Const ReqS in
-    let a = assign (Ident ''CurCmd'', Const ReqS) ||
-            assign (Ident ''CurPtr'', Const (index i)) ||
-            assign (Para ''Chan1.Cmd'' i, Const Empty) ||
-            forallStm (\<lambda>j. assign (Para ''InvSet'' j, IVar (Para ''ShrSet'' j))) N in
-      (guard g a)"
+    IVar (Ident ''CurCmd'') =\<^sub>f Const Empty \<and>\<^sub>f
+    IVar (Para ''Chan1.Cmd'' i) =\<^sub>f Const ReqS
+   \<triangleright>
+    assign (Ident ''CurCmd'', Const ReqS) ||
+    assign (Ident ''CurPtr'', Const (index i)) ||
+    assign (Para ''Chan1.Cmd'' i, Const Empty) ||
+    forallStm (\<lambda>j. assign (Para ''InvSet'' j, IVar (Para ''ShrSet'' j))) N"
+
+lemma symRecvReqS:
+  "symParamRule N (n_RecvReqS N)"
+  unfolding n_RecvReqS_def
+  apply (rule symParamRuleI)
+  subgoal unfolding symParamForm_def by auto
+  subgoal apply (auto intro!: symParamStatementParallel symParamStatementForall)
+    unfolding symParamStatement_def symParamStatement2_def by auto
+  done  
 
 lemma absRecvReqS:
   "absTransfForm M (pre (n_RecvReqS N i)) =
@@ -446,10 +495,14 @@ lemma RecvReqSWellForm:
 
 definition n_SendReqE1 :: "nat \<Rightarrow> rule" where
   "n_SendReqE1 i \<equiv>
-    let g = IVar (Para ''Chan1.Cmd'' i) =\<^sub>f Const Empty \<and>\<^sub>f
-            IVar (Para ''Cache.State'' i) =\<^sub>f Const I in
-    let a = assign (Para ''Chan1.Cmd'' i, Const ReqE) in
-      (guard g a)"
+    IVar (Para ''Chan1.Cmd'' i) =\<^sub>f Const Empty \<and>\<^sub>f
+    IVar (Para ''Cache.State'' i) =\<^sub>f Const I
+   \<triangleright>
+    assign (Para ''Chan1.Cmd'' i, Const ReqE)"
+
+lemma symSendReqE1:
+  "symParamRule N n_SendReqE1"
+  unfolding n_SendReqE1_def symParamRule_def by auto
 
 lemma absSendReqE1:
   "absTransfForm M (pre (n_SendReqE1 i)) =
@@ -474,10 +527,14 @@ lemma SendReqE1WellForm:
 
 definition n_SendReqE2 :: "nat \<Rightarrow> rule" where
   "n_SendReqE2 i \<equiv>
-    let g = IVar (Para ''Chan1.Cmd'' i) =\<^sub>f Const Empty \<and>\<^sub>f
-            IVar (Para ''Cache.State'' i) =\<^sub>f Const S in
-    let a = assign (Para ''Chan1.Cmd'' i, Const ReqE) in
-      (guard g a)"
+    IVar (Para ''Chan1.Cmd'' i) =\<^sub>f Const Empty \<and>\<^sub>f
+    IVar (Para ''Cache.State'' i) =\<^sub>f Const S
+   \<triangleright>
+    assign (Para ''Chan1.Cmd'' i, Const ReqE)"
+
+lemma symSendReqE2:
+  "symParamRule N n_SendReqE2"
+  unfolding n_SendReqE2_def symParamRule_def by auto
 
 lemma absSendReqE2:
   "absTransfForm M (pre (n_SendReqE2 i)) =
@@ -502,10 +559,14 @@ lemma SendReqE2WellForm:
 
 definition n_SendReqS :: "nat \<Rightarrow> rule" where
   "n_SendReqS i \<equiv>
-    let g = IVar (Para ''Chan1.Cmd'' i) =\<^sub>f Const Empty \<and>\<^sub>f
-            IVar (Para ''Cache.State'' i) =\<^sub>f Const I in
-    let a = assign (Para ''Chan1.Cmd'' i, Const ReqS) in
-      (guard g a)"
+    IVar (Para ''Chan1.Cmd'' i) =\<^sub>f Const Empty \<and>\<^sub>f
+    IVar (Para ''Cache.State'' i) =\<^sub>f Const I
+   \<triangleright>
+    assign (Para ''Chan1.Cmd'' i, Const ReqS)"
+
+lemma symSendReqS:
+  "symParamRule N n_SendReqS"
+  unfolding n_SendReqS_def symParamRule_def by auto 
 
 lemma absSendReqS:
   "absTransfForm M (pre (n_SendReqS i)) =
@@ -530,10 +591,10 @@ lemma SendReqSWellForm:
 
 definition n_Store :: "nat \<Rightarrow> rule" where
   "n_Store i \<equiv>
-    let g = IVar (Para ''Cache.State'' i) =\<^sub>f Const E in
-    let a = assign (Para ''Cache.Data'' i, IVar (Ident ''d'')) ||
-            assign (Ident ''AuxData'', IVar (Ident ''d'')) in
-      (guard g a)"
+    IVar (Para ''Cache.State'' i) =\<^sub>f Const E
+   \<triangleright>
+    assign (Para ''Cache.Data'' i, IVar (Ident ''d'')) ||
+    assign (Ident ''AuxData'', IVar (Ident ''d''))"
 
 definition rules :: "nat \<Rightarrow> rule set" where
   "rules N \<equiv> {r.
@@ -605,8 +666,8 @@ definition allInitSpecs :: "nat \<Rightarrow> formula list" where
     initSpec7
   ]"
 
-definition invAux_1 :: "nat \<Rightarrow> nat \<Rightarrow> formula" where
-  "invAux_1 N i \<equiv>
+definition invAux :: "nat \<Rightarrow> nat \<Rightarrow> formula" where
+  "invAux N i \<equiv>
      IVar (Para ''Chan3.Cmd'' i) =\<^sub>f Const InvAck \<and>\<^sub>f
      \<not>\<^sub>f IVar (Ident ''CurCmd'') =\<^sub>f Const Empty \<and>\<^sub>f
      IVar (Ident ''ExGntd'') =\<^sub>f Const true \<longrightarrow>\<^sub>f
@@ -614,30 +675,30 @@ definition invAux_1 :: "nat \<Rightarrow> nat \<Rightarrow> formula" where
      forallFormExcl (\<lambda>j. \<not>\<^sub>f IVar (Para ''Chan2.Cmd'' j) =\<^sub>f Const GntE) i N \<and>\<^sub>f
      forallFormExcl (\<lambda>j. \<not>\<^sub>f IVar (Para ''Chan3.Cmd'' j) =\<^sub>f Const InvAck) i N"
 
-definition n_RecvInvAck1_st :: "nat \<Rightarrow> nat \<Rightarrow> rule" where
-  "n_RecvInvAck1_st N i = strengthenRule2 (invAux_1 N i) (n_RecvInvAck1 i)"
+definition n_RecvInvAck1' :: "nat \<Rightarrow> nat \<Rightarrow> rule" where
+  "n_RecvInvAck1' N i = strengthenRule2 (invAux N i) (n_RecvInvAck1 i)"
 
-definition n_RecvInvAck1_st_ref :: "nat \<Rightarrow> nat \<Rightarrow> rule" where
-  "n_RecvInvAck1_st_ref N i \<equiv>
-    let g =  (IVar (Para ''Chan3.Cmd'' i) =\<^sub>f Const InvAck \<and>\<^sub>f
-              \<not>\<^sub>f IVar (Ident ''CurCmd'') =\<^sub>f Const Empty \<and>\<^sub>f
-              IVar (Ident ''ExGntd'') =\<^sub>f Const true) \<and>\<^sub>f
-             forallFormExcl (\<lambda>j. \<not>\<^sub>f IVar (Para ''Cache.State'' j) =\<^sub>f Const E) i N \<and>\<^sub>f
-             forallFormExcl (\<lambda>j. \<not>\<^sub>f IVar (Para ''Chan2.Cmd'' j) =\<^sub>f Const GntE) i N \<and>\<^sub>f
-             forallFormExcl (\<lambda>j. \<not>\<^sub>f IVar (Para ''Chan3.Cmd'' j) =\<^sub>f Const InvAck) i N in
-    let a = assign (Para ''Chan3.Cmd'' i, Const Empty) ||
-            assign (Para ''ShrSet'' i, Const false) ||
-            assign (Ident ''ExGntd'', Const false) in
-      (guard g a)"
+definition n_RecvInvAck1'_ref :: "nat \<Rightarrow> nat \<Rightarrow> rule" where
+  "n_RecvInvAck1'_ref N i \<equiv>
+    (IVar (Para ''Chan3.Cmd'' i) =\<^sub>f Const InvAck \<and>\<^sub>f
+     \<not>\<^sub>f IVar (Ident ''CurCmd'') =\<^sub>f Const Empty \<and>\<^sub>f
+     IVar (Ident ''ExGntd'') =\<^sub>f Const true) \<and>\<^sub>f
+    forallFormExcl (\<lambda>j. \<not>\<^sub>f IVar (Para ''Cache.State'' j) =\<^sub>f Const E) i N \<and>\<^sub>f
+    forallFormExcl (\<lambda>j. \<not>\<^sub>f IVar (Para ''Chan2.Cmd'' j) =\<^sub>f Const GntE) i N \<and>\<^sub>f
+    forallFormExcl (\<lambda>j. \<not>\<^sub>f IVar (Para ''Chan3.Cmd'' j) =\<^sub>f Const InvAck) i N
+   \<triangleright>
+    assign (Para ''Chan3.Cmd'' i, Const Empty) ||
+    assign (Para ''ShrSet'' i, Const false) ||
+    assign (Ident ''ExGntd'', Const false)"
 
-lemma n_RecvInvAck1_stEq:
-  "n_RecvInvAck1_st N i = n_RecvInvAck1_st_ref N i"
-  by (auto simp add: n_RecvInvAck1_st_def invAux_1_def n_RecvInvAck1_def n_RecvInvAck1_st_ref_def)
+lemma n_RecvInvAck1'Eq:
+  "n_RecvInvAck1' N i = n_RecvInvAck1'_ref N i"
+  by (auto simp add: n_RecvInvAck1'_def invAux_def n_RecvInvAck1_def n_RecvInvAck1'_ref_def)
 
-lemma absRecvInvAck1_st:
+lemma absRecvInvAck1':
   assumes "M \<le> N"
   shows
-  "absTransfForm M (pre (n_RecvInvAck1_st_ref N i)) =
+  "absTransfForm M (pre (n_RecvInvAck1'_ref N i)) =
     (if i > M then
        (\<not>\<^sub>f IVar (Ident ''CurCmd'') =\<^sub>f Const Empty \<and>\<^sub>f
         IVar (Ident ''ExGntd'') =\<^sub>f Const true) \<and>\<^sub>f
@@ -648,7 +709,7 @@ lemma absRecvInvAck1_st:
        IVar (Para ''Chan3.Cmd'' i) =\<^sub>f Const InvAck \<and>\<^sub>f
        \<not>\<^sub>f IVar (Ident ''CurCmd'') =\<^sub>f Const Empty \<and>\<^sub>f
        IVar (Ident ''ExGntd'') =\<^sub>f Const true)"
-  unfolding n_RecvInvAck1_st_ref_def using assms by auto
+  unfolding n_RecvInvAck1'_ref_def using assms by auto
 
 
 end
